experiments/HafniumCore/hfc/MpoolSeq.v
@@ -132,8 +132,8 @@ Simplified Mpool := Vptr [Vptr//chunk_list ; Vptr//fallback]
   (* } *)
 
   Definition init (p: var): stmt :=
-    (Store p chunk_list_ofs Vnull) #;
-    (Store p fallback_ofs Vnull)
+    (p @ chunk_list_ofs #:= Vnull) #;
+    (p @ fallback_ofs   #:= Vnull)
   .
 
   (* void mpool_init_with_fallback(struct mpool *p, struct mpool *fallback) *)
@@ -144,7 +144,7 @@ Simplified Mpool := Vptr [Vptr//chunk_list ; Vptr//fallback]
 
   Definition init_with_fallback (p fallback: var): stmt :=
     Call "init" [CBR p] #;
-    (Store p fallback_ofs fallback)
+    (p @ fallback_ofs #:= fallback)
   .
 
   (* void *mpool_alloc_contiguous(struct mpool *p, size_t count, size_t align) *)
@@ -166,19 +166,16 @@ Simplified Mpool := Vptr [Vptr//chunk_list ; Vptr//fallback]
   Definition alloc_contiguous
              (p count: var)
              (ret: var): stmt :=
-    #if (CoqCode [p: expr] (fun p => mpool_wf (nth 0 p Vnull)))
-     then Skip
-     else Guarantee
-    #;
+    #guarantee (CoqCode [p: expr] (fun p => mpool_wf (nth 0 p Vnull))) #;
     #while Vtrue
      do (
        Debug "looping alloc_contiguous" Vnull #;
-       ret #:= (Call "alloc_contiguous_no_fallback" [CBR p ; CBV count]) #;
+       ret #= (Call "alloc_contiguous_no_fallback" [CBR p ; CBV count]) #;
        #if (ret)
        then (Return ret)
        else Skip
        #;
-       p #:= (Load p fallback_ofs) #;
+       p #= (p #@ fallback_ofs) #;
        #if (p)
        then Skip
        else Break
@@ -190,21 +187,18 @@ Simplified Mpool := Vptr [Vptr//chunk_list ; Vptr//fallback]
   Definition alloc_contiguous2
              (p count: var)
              (ret next nextp: var): stmt :=
-    #if (CoqCode [p: expr] (fun p => mpool_wf (nth 0 p Vnull)))
-     then Skip
-     else Guarantee
-    #;
-    next #:= (Load p chunk_list_ofs) #;
-    ret #:= (Call "alloc_contiguous_no_fallback2" [CBR next ; CBV count]) #;
-    Store p chunk_list_ofs next #;
+    #guarantee (CoqCode [p: expr] (fun p => mpool_wf (nth 0 p Vnull))) #;
+    next #= (p #@ chunk_list_ofs) #;
+    ret #= (Call "alloc_contiguous_no_fallback2" [CBR next ; CBV count]) #;
+    p @ chunk_list_ofs #:= next #;
     #if (ret)
      then (Return ret)
      else (
-         nextp #:= (Load p fallback_ofs) #;
+         nextp #= (p #@ fallback_ofs) #;
          #if (! nextp) then Return Vnull else Skip #;
          (* Put "Looking inside fallback.." Vnull #; *)
-         ret #:= (Call "alloc_contiguous2" [CBR nextp ; CBV count]) #;
-         (Store p fallback_ofs nextp) #;
+         ret #= (Call "alloc_contiguous2" [CBR nextp ; CBV count]) #;
+         (p @ fallback_ofs #:= nextp) #;
          Return ret
        )
   .
@@ -259,42 +253,39 @@ Simplified Mpool := Vptr [Vptr//chunk_list ; Vptr//fallback]
   Definition alloc_contiguous_no_fallback
              (p count: var)
              (prev ret new_chunk chunk: var): stmt :=
-    #if (CoqCode [p: expr] (fun p => mpool_wf (nth 0 p Vnull)))
-     then Skip
-     else Guarantee
-    #;
-    prev #:= (#& (Load p chunk_list_ofs)) #;
+    #guarantee (CoqCode [p: expr] (fun p => mpool_wf (nth 0 p Vnull))) #;
+    prev #= (#& (p #@ chunk_list_ofs)) #;
     Debug "(A)prev_is: " prev #;
     #while prev
      do (
-       chunk #:= (#* prev) #;
-       new_chunk #:= (SubPointerFrom chunk (count * entry_size)) #;
+       chunk #= (#* prev) #;
+       new_chunk #= (SubPointerFrom chunk (count * entry_size)) #;
        (* if (new_chunk <= chunk->limit) *)
        (* #if new_chunk *)
-       #if (count <= (Load chunk limit_ofs))
+       #if (count <= (chunk #@ limit_ofs))
         then
           (
-           (Debug "If1-limit: " (Load chunk limit_ofs)) #;
-           #if count == (Load chunk limit_ofs)
+           (Debug "If1-limit: " (chunk #@ limit_ofs)) #;
+           #if count == (chunk #@ limit_ofs)
             then (
-                Store prev 0 (Load chunk next_chunk_ofs) (** should write to p **)
+                prev @ 0 #:= (chunk #@ next_chunk_ofs) (** should write to p **)
               )
             else (
-                Store new_chunk next_chunk_ofs (Load chunk next_chunk_ofs) #;
-                Store new_chunk limit_ofs (Load chunk limit_ofs) #;
-                Store prev 0 new_chunk
+                new_chunk @ next_chunk_ofs #:= (chunk #@ next_chunk_ofs) #;
+                new_chunk @ limit_ofs #:= (chunk #@ limit_ofs) #;
+                prev @ 0 #:= new_chunk
               )
            #;
            (* ret = (void * )start; *) (** code doesn't specify the size, but we need too **)
            Debug "(A)chunk_is: " chunk #;
-           ret #:= (SubPointerTo chunk (count * entry_size)) #;
+           ret #= (SubPointerTo chunk (count * entry_size)) #;
            Debug "(A)ret_is: " ret #;
            Break
           )
         else
           (
-            (Debug "Else1-limit: " (Load chunk limit_ofs)) #;
-            (prev #:= #& (Load chunk next_chunk_ofs)) #;
+            (Debug "Else1-limit: " (chunk #@ limit_ofs)) #;
+            (prev #= #& (chunk #@ next_chunk_ofs)) #;
             (Debug "Else1-prev: " prev) #;
             Skip
           )
@@ -308,32 +299,32 @@ Simplified Mpool := Vptr [Vptr//chunk_list ; Vptr//fallback]
              (cur count: var)
              (ret next cur_ofs new_cur: var): stmt :=
     #if ! cur then Return Vnull else Skip #;
-    cur_ofs #:= (Load cur limit_ofs) #;
+    cur_ofs #= (cur #@ limit_ofs) #;
     #if (count <= cur_ofs)
      then (
            (* (Debug "If-limit: " cur_ofs) #; *)
            #if count == cur_ofs
             then (
                 (* (Debug "If-If: " Vnull) #; *)
-                ret #:= (SubPointerTo cur (count * entry_size)) #;
-                cur #:= (Load cur next_chunk_ofs) #;
+                ret #= (SubPointerTo cur (count * entry_size)) #;
+                cur #= (cur #@ next_chunk_ofs) #;
                 Return ret
               )
             else (
                 (* (Debug "If-Else: " Vnull) #; *)
-                new_cur #:= (SubPointerFrom cur (count * entry_size)) #;
-                Store new_cur next_chunk_ofs (Load cur next_chunk_ofs) #;
-                Store new_cur limit_ofs (cur_ofs - count) #;
-                ret #:= (SubPointerTo cur (count * entry_size)) #;
-                cur #:= new_cur #;
+                new_cur #= (SubPointerFrom cur (count * entry_size)) #;
+                new_cur @ next_chunk_ofs #:= (cur #@ next_chunk_ofs) #;
+                new_cur @ limit_ofs #:= (cur_ofs - count) #;
+                ret #= (SubPointerTo cur (count * entry_size)) #;
+                cur #= new_cur #;
                 Return ret
               )
           )
      else (
          (* (Debug "Else-limit: " cur_ofs) #; *)
-         next #:= (Load cur next_chunk_ofs) #;
-         ret #:= (Call "alloc_contiguous_no_fallback2" [CBR next ; CBV count]) #;
-         Store cur next_chunk_ofs next #;
+         next #= (cur #@ next_chunk_ofs) #;
+         ret #= (Call "alloc_contiguous_no_fallback2" [CBR next ; CBV count]) #;
+         cur @ next_chunk_ofs #:= next #;
          Return ret
          )
   .
@@ -369,31 +360,29 @@ Simplified Mpool := Vptr [Vptr//chunk_list ; Vptr//fallback]
   Definition add_chunk
              (p begin size: var)
              (chunk: var): stmt :=
-    chunk #:= begin #;
+    chunk #= begin #;
     (* Store chunk limit_ofs ((GetLen chunk) / entry_size) #; *)
-    Store chunk limit_ofs size #;
+    chunk @ limit_ofs #:= size #;
 
-    Store chunk next_chunk_ofs (Load p chunk_list_ofs) #;
-    Store p chunk_list_ofs chunk
+    chunk @ next_chunk_ofs #:= (p #@ chunk_list_ofs) #;
+    p @ chunk_list_ofs #:= chunk
   .
 
-  Definition initF: function :=
-    mk_function ["p"] (init "p").
-  Definition init_with_fallbackF: function :=
-    mk_function ["p" ; "fb"] (init_with_fallback "p" "fb").
-  Definition alloc_contiguousF: function :=
-    mk_function ["p" ; "count"] (alloc_contiguous "p" "count" "ret").
-  Definition alloc_contiguous_no_fallbackF: function :=
-    mk_function ["p" ; "count"]
-                (alloc_contiguous_no_fallback "p" "count" "prev" "ret" "new_chunk" "chunk").
-  Definition alloc_contiguous2F: function :=
-    mk_function ["p" ; "count"] (alloc_contiguous2 "p" "count" "ret" "next" "nextp").
-  Definition alloc_contiguous_no_fallback2F: function :=
-    mk_function ["cur" ; "count"]
-                (alloc_contiguous_no_fallback2 "cur" "count" "ret" "next"
-                                               "cur_ofs" "new_cur").
-  Definition add_chunkF: function :=
-    mk_function ["p" ; "begin" ; "size"] (add_chunk "p" "begin" "size" "chunk").
+  Definition initF: function. mk_function_tac init ["p"] ([]: list var). Defined.
+  Definition init_with_fallbackF: function.
+    mk_function_tac init_with_fallback ["p" ; "fb"] ([]: list var). Defined.
+  Definition alloc_contiguousF: function.
+    mk_function_tac alloc_contiguous ["p" ; "count"] ["ret"]. Defined.
+  Definition alloc_contiguous_no_fallbackF: function.
+    mk_function_tac alloc_contiguous_no_fallback
+                    ["p" ; "count"] ["prev" ; "ret" ; "new_chunk" ; "chunk"]. Defined.
+  Definition alloc_contiguous2F: function.
+    mk_function_tac alloc_contiguous2 ["p" ; "count"] ["ret" ; "next" ; "nextp"]. Defined.
+  Definition alloc_contiguous_no_fallback2F: function.
+    mk_function_tac alloc_contiguous_no_fallback2
+                    ["cur" ; "count"] ["ret" ; "next" ; "cur_ofs" ; "new_cur" ]. Defined.
+  Definition add_chunkF: function.
+    mk_function_tac add_chunk ["p" ; "begin" ; "size"] ["chunk"]. Defined.
 
 End MPOOLSEQ.
 
@@ -410,30 +399,31 @@ Module TEST.
 
     Definition main
                (p r1 r2 r3: var): stmt :=
-      p #:= Vptr None [0: val ; 0: val] #;
+      p #= Vptr None [0: val ; 0: val] #;
         (Put "before init: " p) #;
         Call "init" [CBR p] #;
         (Put "after init: " p) #;
         Call "add_chunk" [CBR p ; CBV (big_chunk 500 10) ; CBV 10] #;
         (Put "add_chunk done: " p) #;
 
-        r1 #:= Call "alloc_contiguous" [CBR p ; CBV 7] #;
+        r1 #= Call "alloc_contiguous" [CBR p ; CBV 7] #;
         (Put "alloc first; should succeed: " r1) #;
         (Put "alloc first; p: " p) #;
 
-        r2 #:= Call "alloc_contiguous" [CBR p ; CBV 7] #;
+        r2 #= Call "alloc_contiguous" [CBR p ; CBV 7] #;
         (Put "alloc second; should fail: " r2) #;
         (Put "alloc second; p: " p) #;
 
         Call "add_chunk" [CBR p ; CBV r1 ; CBV 7] #;
         (Put "add_chunk done" p) #;
 
-        r3 #:= Call "alloc_contiguous" [CBR p ; CBV 7] #;
+        r3 #= Call "alloc_contiguous" [CBR p ; CBV 7] #;
         (Put "alloc third; should succeed: " r3) #;
         (Put "alloc third; p: " p) #;
         Skip
     .
-    Definition mainF: function := mk_function [] (main "p" "r1" "r2" "r3").
+    Definition mainF: function.
+      mk_function_tac main ([]: list var) ["p" ; "r1" ; "r2" ; "r3"]. Defined.
 
     Definition program: program :=
       [
@@ -452,36 +442,37 @@ Module TEST.
 
     Definition main
                (p r1 r2 r3: var): stmt :=
-      p #:= Vptr None [0: val ; 0: val] #;
-        (* (Put "before init: " p) #; *)
+      p #= Vptr None [0: val ; 0: val] #;
+        (Debug "before init: " p) #;
         Call "init" [CBR p] #;
-        (* (Put "after init: " p) #; *)
+        (Debug "after init: " p) #;
         Call "add_chunk" [CBR p ; CBV (big_chunk 500 10) ; CBV 10] #;
-        (* (Put "add_chunk done: " p) #; *)
+        (Debug "add_chunk done: " p) #;
 
-        r1 #:= Call "alloc_contiguous2" [CBR p ; CBV 7] #;
-        (* (Put "alloc first; should succeed: " r1) #; *)
-        (* (Put "alloc first; p: " p) #; *)
-        #if r1 then Skip else Assume #;
+        r1 #= Call "alloc_contiguous2" [CBR p ; CBV 7] #;
+        (Debug "alloc first; should succeed: " r1) #;
+        (Debug "alloc first; p: " p) #;
+        #assume r1 #;
 
-        r2 #:= Call "alloc_contiguous2" [CBR p ; CBV 7] #;
-        (* (Put "alloc second; should fail: " r2) #; *)
-        (* (Put "alloc second; p: " p) #; *)
-        #if r2 then Assume else Skip #;
+        r2 #= Call "alloc_contiguous2" [CBR p ; CBV 7] #;
+        (Debug "alloc second; should fail: " r2) #;
+        (Debug "alloc second; p: " p) #;
+        #assume (!r2) #;
 
         Call "add_chunk" [CBR p ; CBV r1 ; CBV 7] #;
-        (* (Put "add_chunk done" p) #; *)
+        (Debug "add_chunk done" p) #;
 
-        r3 #:= Call "alloc_contiguous2" [CBR p ; CBV 7] #;
-        (* (Put "alloc third; should succeed: " r3) #; *)
-        (* (Put "alloc third; p: " p) #; *)
-        #if r3 then Skip else Assume #;
+        r3 #= Call "alloc_contiguous2" [CBR p ; CBV 7] #;
+        (Debug "alloc third; should succeed: " r3) #;
+        (Debug "alloc third; p: " p) #;
+        #assume r3 #;
 
 
         Put "Test2 Passed" Vnull #;
         Skip
     .
-    Definition mainF: function := mk_function [] (main "p" "r1" "r2" "r3").
+    Definition mainF: function.
+      mk_function_tac main ([]: list var) ["p" ; "r1" ; "r2" ; "r3"]. Defined.
 
     Definition program: program :=
       [
@@ -504,7 +495,7 @@ Module TEST.
 
     Definition main
                (p r1 r2 r3: var): stmt :=
-      p #:= Vptr None [0: val ; 0: val] #;
+      p #= Vptr None [0: val ; 0: val] #;
         (* (Put "before init: " p) #; *)
         Call "init" [CBR p] #;
         (* (Put "after init: " p) #; *)
@@ -512,20 +503,21 @@ Module TEST.
         Call "add_chunk" [CBR p ; CBV (big_chunk 1500 10) ; CBV 10] #;
         (* (Put "add_chunk done: " p) #; *)
 
-        r1 #:= Call "alloc_contiguous2" [CBR p ; CBV 7] #;
+        r1 #= Call "alloc_contiguous2" [CBR p ; CBV 7] #;
         (* (Put "alloc first; should succeed: " r1) #; *)
         (* (Put "alloc first; p: " p) #; *)
-        #if r1 then Skip else Assume #;
+        #assume r1 #;
 
-        r2 #:= Call "alloc_contiguous2" [CBR p ; CBV 7] #;
+        r2 #= Call "alloc_contiguous2" [CBR p ; CBV 7] #;
         (* (Put "alloc second; should succeed: " r2) #; *)
         (* (Put "alloc second; p: " p) #; *)
-        #if r2 then Skip else Assume #;
+        #assume r2 #;
 
         Put "Test3 Passed" Vnull #;
         Skip
     .
-    Definition mainF: function := mk_function [] (main "p" "r1" "r2" "r3").
+    Definition mainF: function.
+      mk_function_tac main ([]: list var) ["p" ; "r1" ; "r2" ; "r3"]. Defined.
 
     Definition program: program :=
       [
@@ -546,9 +538,9 @@ Module TEST.
 
     Definition main
                (p0 p1 p2 r: var): stmt :=
-      (* p0 #:= Vptr None [0: val ; 0: val] #; *)
-      (* p1 #:= Vptr None [0: val ; 0: val] #; *)
-      (* p2 #:= Vptr None [0: val ; 0: val] #; *)
+      (* p0 #= Vptr None [0: val ; 0: val] #; *)
+      (* p1 #= Vptr None [0: val ; 0: val] #; *)
+      (* p2 #= Vptr None [0: val ; 0: val] #; *)
       (* Call "init" [CBR p2] #; *)
       (* Call "init_with_fallback" [CBR p1 ; CBV p2] #; *)
       (* Call "init_with_fallback" [CBR p0 ; CBV p1] #; *)
@@ -557,22 +549,22 @@ Module TEST.
       (* Call "add_chunk" [CBR p1 ; CBV (big_chunk 1500 15) ; CBV 15] #; *)
       (* Call "add_chunk" [CBR p2 ; CBV (big_chunk 2500 10) ; CBV 10] #; *)
 
-      (* r #:= Call "alloc_contiguous2" [CBR p0 ; CBV 5] #; *)
-      (* #if r then Skip else Assume #; *)
+      (* r #= Call "alloc_contiguous2" [CBR p0 ; CBV 5] #; *)
+      (* #assume r #; *)
       (* Call "alloc_contiguous2" [CBR p0 ; CBV 10] #; *)
-      (* #if r then Skip else Assume #; *)
+      (* #assume r #; *)
       (* Call "alloc_contiguous2" [CBR p0 ; CBV 15] #; *)
-      (* #if r then Assume else Skip #; *)
+      (* #assume (!r) #; *)
       (* Call "alloc_contiguous2" [CBR p0 ; CBV 5] #; *)
-      (* #if r then Skip else Assume #; *)
+      (* #assume r #; *)
       (* Call "alloc_contiguous2" [CBR p0 ; CBV 10] #; *)
-      (* #if r then Skip else Assume #; *)
+      (* #assume r #; *)
       (* Call "alloc_contiguous2" [CBR p0 ; CBV 5] #; *)
-      (* #if r then Skip else Assume #; *)
+      (* #assume r #; *)
       (* Skip *)
-      p0 #:= Vptr None [0: val ; 0: val] #;
-      p1 #:= Vptr None [0: val ; 0: val] #;
-      p2 #:= Vptr None [0: val ; 0: val] #;
+      p0 #= Vptr None [0: val ; 0: val] #;
+      p1 #= Vptr None [0: val ; 0: val] #;
+      p2 #= Vptr None [0: val ; 0: val] #;
       Call "init" [CBR p2] #;
       Call "add_chunk" [CBR p2 ; CBV (big_chunk 2500 2) ; CBV 2] #;
 
@@ -583,22 +575,23 @@ Module TEST.
       Call "add_chunk" [CBR p0 ; CBV (big_chunk 500  1) ; CBV 1] #;
       
 
-      r #:= Call "alloc_contiguous2" [CBR p0 ; CBV 1] #;
-      #if r then Skip else Assume #;
-      r #:= Call "alloc_contiguous2" [CBR p0 ; CBV 2] #;
-      #if r then Skip else Assume #;
-      r #:= Call "alloc_contiguous2" [CBR p0 ; CBV 3] #;
-      #if r then Assume else Skip #;
-      r #:= Call "alloc_contiguous2" [CBR p0 ; CBV 2] #;
-      #if r then Skip else Assume #;
-      r #:= Call "alloc_contiguous2" [CBR p0 ; CBV 1] #;
-      #if r then Skip else Assume #;
-      r #:= Call "alloc_contiguous2" [CBR p0 ; CBV 1] #;
-      #if r then Assume else Skip #;
+      r #= Call "alloc_contiguous2" [CBR p0 ; CBV 1] #;
+      #assume r #;
+      r #= Call "alloc_contiguous2" [CBR p0 ; CBV 2] #;
+      #assume r #;
+      r #= Call "alloc_contiguous2" [CBR p0 ; CBV 3] #;
+      #assume (!r) #;
+      r #= Call "alloc_contiguous2" [CBR p0 ; CBV 2] #;
+      #assume r #;
+      r #= Call "alloc_contiguous2" [CBR p0 ; CBV 1] #;
+      #assume r #;
+      r #= Call "alloc_contiguous2" [CBR p0 ; CBV 1] #;
+      #assume (!r) #;
       Put "Test4 Passed" Vnull #;
       Skip
     .
-    Definition mainF: function := mk_function [] (main "p0" "p1" "p2" "r").
+    Definition mainF: function.
+      mk_function_tac main ([]: list var) ["p" ; "r1" ; "r2" ; "r3"]. Defined.
 
     Definition program: program :=
       [
@@ -657,9 +650,9 @@ Module TEST.
 
     Definition main
                (p0 p1 p2 q tmp0 tmp1: var): stmt :=
-      p0 #:= Vptr None [0: val ; 0: val] #;
-      p1 #:= Vptr None [0: val ; 0: val] #;
-      p2 #:= Vptr None [0: val ; 0: val] #;
+      p0 #= Vptr None [0: val ; 0: val] #;
+      p1 #= Vptr None [0: val ; 0: val] #;
+      p2 #= Vptr None [0: val ; 0: val] #;
       Call "init" [CBR p0] #;
       Call "init_with_fallback" [CBR p1 ; CBV p0] #;
       Call "init_with_fallback" [CBR p2 ; CBV p1] #;
@@ -669,8 +662,8 @@ Module TEST.
         #if ((CoqCode [] (fun _ => random_range 2)) == 0)
          then
            (* add_chunk *)
-           tmp0 #:= (CoqCode [] (fun _ => random_range 3)) #;
-           tmp1 #:= (CoqCode [] (fun _ => random_range 10)) #;
+           tmp0 #= (CoqCode [] (fun _ => random_range 3)) #;
+           tmp1 #= (CoqCode [] (fun _ => random_range 10)) #;
            (#if (tmp0 == 0)
              then Call "add_chunk" [CBR p0 ; CBV (big_chunk 0 random_latest) ; CBV tmp1]
              else
@@ -679,7 +672,7 @@ Module TEST.
              else
            (#if (tmp0 == 2)
              then Call "add_chunk" [CBR p2 ; CBV (big_chunk 0 random_latest) ; CBV tmp1]
-             else Guarantee)))
+             else #guarantee #false)))
          else
            (* alloc_continuous *)
            Skip
