experiments/HafniumCore/lang/LangTest.v
@@ -59,34 +59,38 @@ Set Implicit Arguments.
 
 
 
+
+
+
+
 Module LoadStore.
 
   Definition main x sum: stmt :=
-    sum #:= Vnat 0#;
-        x #:= Vptr None (repeat (Vnat 0) 3)#;
-        #put x#;
-        (Store x 0 10)#;
-        #put x#;
-        (Store x 1 20)#;
-        #put x#;
-        (Store x 2 30)#;
-        #put x#;
-        #put sum#;
-        sum #:= sum + (Load x 0)#;
-                                #put sum#;
-                                sum #:= sum + (Load x 1)#;
-                                                        #put sum#;
-                                                        sum #:= sum + (Load x 2)#;
-                                                                                #put sum#;
-                                                                                Skip
+    sum #= Vnat 0#;
+    x #= Vptr None (repeat (Vnat 0) 3)#;
+    Put "" x#;
+    (x @ 0 #:= 10)#;
+    Put "" x#;
+    (x @ 1 #:= 20)#;
+    Put "" x#;
+    (x @ 2 #:= 30)#;
+    Put "" x#;
+    Put "" sum#;
+    sum #= sum + (x #@ 0)#;
+    Put "" sum#;
+    sum #= sum + (x #@ 1)#;
+    Put "" sum#;
+    sum #= sum + (x #@ 2)#;
+    Put "" sum#;
+    Skip
   .
 
-  Definition function: function := mk_function [] (main "x" "sum").
+  Definition function: function. mk_function_tac main ([]: list var) ["x" ; "sum"]. Defined.
 
   Definition program: program := [("main", function)].
 
   (* Extraction "LangTest.ml" load_store_program. *)
-  Check (eval_program program).
+  Check (eval_whole_program program).
 
 End LoadStore.
 
@@ -95,10 +99,10 @@ Section TMP.
   Variable a: var.
   Variable b: val.
   Check (Var a).
-  Check (Lit b).
+  Check (Val b).
   Local Open Scope expr_scope.
   Local Open Scope stmt_scope.
-  Check ((Var a) + (Lit b)).
+  Check ((Var a) + (Val b)).
 End TMP.
 
 Local Open Scope expr_scope.
@@ -109,24 +113,25 @@ Module Rec.
 
   Definition f x y r: stmt :=
     (#if x
-      then (y #:= (x - 1) #;
-              r #:= (Call "f" [CBV y]) #;
-              r #:= r + x)
-      else (r #:= 0)
+      then (y #= (x - 1) #;
+              r #= (Call "f" [CBV y]) #;
+              r #= r + x)
+      else (r #= 0)
     )
       #;
       Return r
   .
 
-  Definition f_function: function := mk_function ["x"] (f "x" "local0" "local1").
+  Definition f_function: function. mk_function_tac f ["x"] ["local0" ; "local1"]. Defined.
 
   Definition main x r: stmt :=
-    x #:= 10 #;
-      r #:= (Call "f" [CBV x]) #;
-      #put r
+    x #= 10 #;
+      r #= (Call "f" [CBV x]) #;
+      Put "" r
   .
 
-  Definition main_function: function := mk_function [] (main "local0" "local1").
+  Definition main_function: function.
+    mk_function_tac main ([]:list var) ["local0" ; "local1"]. Defined.
 
   Definition program: program := [("main", main_function) ;
                                     ("f", f_function)].
@@ -139,10 +144,10 @@ Module MutRec.
 
   Definition f x y r: stmt :=
     (#if x
-      then (y #:= (x - 1) #;
-              r #:= (Call "g" [CBV y]) #;
-              r #:= r + x)
-      else (r #:= 0)
+      then (y #= (x - 1) #;
+              r #= (Call "g" [CBV y]) #;
+              r #= r + x)
+      else (r #= 0)
     )
       #;
       Return r
@@ -150,17 +155,17 @@ Module MutRec.
 
   Definition g x y r: stmt :=
     (#if x
-      then (y #:= (x - 1) #;
-              r #:= (Call "f" [CBV y]) #;
-              r #:= r + x)
-      else (r #:= 0)
+      then (y #= (x - 1) #;
+              r #= (Call "f" [CBV y]) #;
+              r #= r + x)
+      else (r #= 0)
     )
       #;
       Return r
   .
 
-  Definition f_function: function := mk_function ["x"] (f "x" "local0" "local1").
-  Definition g_function: function := mk_function ["x"] (g "x" "local0" "local1").
+  Definition f_function: function. mk_function_tac f ["x"] ["local0" ; "local1"]. Defined.
+  Definition g_function: function. mk_function_tac g ["x"] ["local0" ; "local1"]. Defined.
 
   Definition program: program := [("main", Rec.main_function) ;
                                     ("f", f_function) ;
@@ -172,33 +177,33 @@ End MutRec.
 (* YJ: if we just use "r", not "unused", something weird will happen *)
 (* TODO: address it better *)
 Module Move.
-  Definition f (x y accu unused: var): stmt :=
+  Definition f (x accu y unused: var): stmt :=
     (#if x
-      then (y #:= (x - 1) #;
+      then (y #= (x - 1) #;
               (* Put "before call" accu #; *)
-              unused #:= (Call "f" [CBV y ; CBR accu]) #;
+              unused #= (Call "f" [CBV y ; CBR accu]) #;
               (* Put "after call" accu #; *)
-              accu #:= accu + x #;
+              accu #= accu + x #;
                                 Skip
            )
       else
-        (accu #:= 0)
+        (accu #= 0)
     )
       #;
       Return 77777
   .
 
   Definition main x accu unused: stmt :=
-    x #:= 10 #;
-      accu #:= 1000 #;
-      unused #:= (Call "f" [CBV x ; CBR accu]) #;
-      #put accu
+    x #= 10 #;
+      accu #= 1000 #;
+      unused #= (Call "f" [CBV x ; CBR accu]) #;
+      Put "" accu
   .
 
-  Definition f_function: function := mk_function ["x" ; "accu"]
-                                                      (f "x" "local0" "accu" "local1").
-  Definition main_function: function :=
-    mk_function [] (main "local0" "local1" "local2").
+  Definition f_function: function. mk_function_tac f ["x" ; "accu"]
+                                                   ["local0" ; "local1"]. Defined.
+  Definition main_function: function.
+    mk_function_tac main ([]:list var) ["local0" ; "local1" ; "local2"]. Defined.
 
   Definition program: program := [("main", main_function) ;
                                     ("f", f_function)].
@@ -227,14 +232,14 @@ Module CoqCode.
   Extract Constant coqcode => "fun _ -> coq_Vtrue".
 
   Definition main x: stmt :=
-    x #:= 25 #;
+    x #= 25 #;
       (#if (CoqCode [Var x] coqcode)
-        then #put 555
-        else #put 666)
+        then Put "" 555
+        else Put "" 666)
   .
 
-  Definition main_function: function :=
-    mk_function [] (main "local0").
+  Definition main_function: function.
+    mk_function_tac main ([]: list var) ["local0"]. Defined.
 
   Definition program: program := [("main", main_function)].
 
@@ -245,47 +250,45 @@ End CoqCode.
 Module Control.
 
   Definition f ctrl ret iter: stmt :=
-    iter #:= 10 #;
-    ret #:= 0 #;
-    (* #put ctrl #; *)
-    (* #put iter #; *)
-    (* #put ret #; *)
-    (* #put 7777777 #; *)
+    iter #= 10 #;
+    ret #= 0 #;
+    (* Put "" ctrl #; *)
+    (* Put "" iter #; *)
+    (* Put "" ret #; *)
+    (* Put "" 7777777 #; *)
     #while iter
      do (
-          iter #:= iter - 1#;
+          iter #= iter - 1#;
           (* 0 --> break *)
           (* 1 --> continue *)
           (* 2 --> return *)
           (* 3 --> normal *)
           #if ctrl == 0 then Break else Skip #;
-          (* #put 1111 #; *)
-          ret #:= ret + 1 #;
+          (* Put "" 1111 #; *)
+          ret #= ret + 1 #;
           #if ctrl == 1 then Continue else Skip #;
-          (* #put 2222 #; *)
-          ret #:= ret + 10 #;
+          (* Put "" 2222 #; *)
+          ret #= ret + 10 #;
           #if ctrl == 2 then (Return (ret + 100)) else Skip #;
-          (* #put 3333 #; *)
-          ret #:= ret + 1000 #;
+          (* Put "" 3333 #; *)
+          ret #= ret + 1000 #;
 
           Skip
           ) #;
      Return ret
   .
 
-  Definition f_function: function := mk_function ["ctrl"] (f "ctrl" "local0" "local1").
+  Definition f_function: function. mk_function_tac f ["ctrl"] ["local0" ; "local1"]. Defined.
 
   Definition main r: stmt :=
-    r #:= (Call "f" [CBV 0]) #; #if r == 0 then Skip else Assume #;
-    r #:= (Call "f" [CBV 1]) #; #if r == 10 then Skip else Assume #;
-    r #:= (Call "f" [CBV 2]) #; #if r == 111 then Skip else Assume #;
-    r #:= (Call "f" [CBV 3]) #; #if r == 10110 then Skip else Assume #;
+    r #= (Call "f" [CBV 0]) #; #assume (r == 0) #;
+    r #= (Call "f" [CBV 1]) #; #assume (r == 10) #;
+    r #= (Call "f" [CBV 2]) #; #assume (r == 111) #;
+    r #= (Call "f" [CBV 3]) #; #assume (r == 10110) #;
     Skip
   .
 
-  Definition main_function: function :=
-    mk_function [] (main "local0")
-  .
+  Definition main_function: function. mk_function_tac main ([]: list var) ["local0"]. Defined.
 
   Definition program: program := [("main", main_function) ;
                                     ("f", f_function)].
@@ -301,17 +304,15 @@ Module DoubleReturn.
     Return 0 #; Return 1
   .
 
-  Definition f_function: function := mk_function [] f.
+  Definition f_function: function. mk_function_tac f ([]: list var) ([]: list var). Defined.
 
   Definition main r :=
-    r #:= (Call "f" []) #;
-    #if ! (r == 0) then Assume else Skip #;
+    r #= (Call "f" []) #;
+    #assume (r == 0) #;
     Skip
   .
 
-  Definition main_function: function :=
-    mk_function [] (main "local0")
-  .
+  Definition main_function: function. mk_function_tac main ([]: list var) ["local0"]. Defined.
 
   Definition program: program := [("main", main_function) ;
                                     ("f", f_function)].
@@ -324,20 +325,19 @@ End DoubleReturn.
 Module MultiCore.
 
   Definition main (n: nat): stmt :=
-    #put (n + 1) #;
-    #put (n + 2) #;
+    Put "" (n + 1) #;
+    Put "" (n + 2) #;
     Yield #;
-    #put (n + 3) #;
-    #put (n + 4) #;
+    Put "" (n + 3) #;
+    Put "" (n + 4) #;
     Yield #;
-    #put (n + 5) #;
-    #put (n + 6) #;
+    Put "" (n + 5) #;
+    Put "" (n + 6) #;
     Skip
   .
 
-  Definition main_function n: function :=
-    mk_function [] (main n)
-  .
+  Definition main_function (n: nat): function.
+    mk_function_tac (main n) ([]: list var) ([]: list var). Defined.
 
   Definition program n: program := [("main", main_function n) ].
 
@@ -348,14 +348,115 @@ End MultiCore.
 
 
 
+
+Module MultiCore2.
+
+  Definition observer i: stmt :=
+    i #= 20 #;
+    #while i
+    do (
+      i #= i -1 #;
+      #assume ("GVAR" % 2 == 0) #;
+      Yield
+    ) #;
+    #if "GVAR" == 0 then AssumeFail else Skip #; (* Test if GlobalE actually worked *)
+    Put "Test(MultiCore2) passed" Vnull
+  .
+
+  Definition adder i: stmt :=
+    i #= 20 #;
+    #while i
+    do (
+      i #= i - 1 #;
+      "GVAR" #= "GVAR" + 1 #;
+      "GVAR" #= "GVAR" + 1 #;
+      Yield
+    )
+  .
+
+  (* Definition main: stmt := *)
+  (*   "GVAR" #:= 10 #; Yield *)
+  (* . *)
+
+  Definition observerF: function. mk_function_tac observer ([]: list var) (["i"]). Defined.
+  Definition adderF: function. mk_function_tac adder ([]: list var) (["i"]). Defined.
+  (* Definition mainF: function. mk_function_tac main ([]: list var) ([]: list var). Defined. *)
+
+  Definition observerP: program := [("main", observerF) ].
+  Definition adderP: program := [("main", adderF) ].
+  (* Definition mainP: program := [("main", mainF) ]. *)
+
+  (* Definition programs: list Lang.program := [ observerP ; adderP ; adderP ; mainP ]. *)
+  Definition programs: list Lang.program := [ observerP ; adderP ; adderP ].
+
+  Definition sem :=
+   ITree.ignore
+     (interp_GlobalE (round_robin (List.map eval_single_program programs)) []).
+
+End MultiCore2.
+
+
+
+
+
+
+Module MultiCoreMPSC.
+
+  Definition producer i: stmt :=
+    i #= 10 #;
+    #while i
+    do (
+      Debug "PRODUCER: " i #;
+      #if "GVAR" == 0
+       then ("GVAR" #= i #; i #= i-1)
+       else Skip #;
+      Yield
+    ) #;
+    "SIGNAL" #= "SIGNAL" + 1
+  .
+
+  Definition consumer s: stmt :=
+    s #= 0 #;
+    #while true
+    do (
+      Debug "CONSUMER: " s #;
+      #if "GVAR" == 0
+       then Skip
+       else s #= s + "GVAR" #;
+            "GVAR" #= 0
+      #;
+      #if "SIGNAL" == 2 then Break else Skip #;
+      Yield
+    ) #;
+    (* Put "" s #; *)
+    #assume (s == 110) #;
+    Put "Test(MultiCore3) passed" Vnull
+  .
+
+  Definition producerF: function. mk_function_tac producer ([]: list var) (["i"]). Defined.
+  Definition consumerF: function. mk_function_tac consumer ([]: list var) (["s"]). Defined.
+
+  Definition producerP: program := [("main", producerF) ].
+  Definition consumerP: program := [("main", consumerF) ].
+
+  Definition programs: list Lang.program := [ producerP ; consumerP ; producerP ].
+
+  Definition sem :=
+   ITree.ignore
+     (interp_GlobalE (round_robin (List.map eval_single_program programs)) []).
+
+End MultiCoreMPSC.
+
+
+
 Module MultiModule.
 
   Definition f x y r: stmt :=
     (#if x
-      then (y #:= (x - 1) #;
-              r #:= (Call "g" [CBV y]) #;
-              r #:= r + x)
-      else (r #:= 0)
+      then (y #= (x - 1) #;
+              r #= (Call "g" [CBV y]) #;
+              r #= r + x)
+      else (r #= 0)
     )
     #;
     Return r
@@ -363,17 +464,17 @@ Module MultiModule.
 
   Definition g x y r: stmt :=
     (#if x
-      then (y #:= (x - 1) #;
-              r #:= (Call "f" [CBV y]) #;
-              r #:= r + x)
-      else (r #:= 0)
+      then (y #= (x - 1) #;
+              r #= (Call "f" [CBV y]) #;
+              r #= r + x)
+      else (r #= 0)
     )
     #;
     Return r
   .
 
-  Definition f_function: function := mk_function ["x"] (f "x" "local0" "local1").
-  Definition g_function: function := mk_function ["x"] (g "x" "local0" "local1").
+  Definition f_function: function. mk_function_tac f ["x"] ["local0" ; "local1"]. Defined.
+  Definition g_function: function. mk_function_tac g ["x"] ["local0" ; "local1"]. Defined.
 
   Definition main_program: program := [("main", Rec.main_function)].
   Definition f_program: program := [("f", f_function)].
@@ -388,13 +489,53 @@ End MultiModule.
 
 
 
+
+Module MultiModuleGenv.
+
+  Definition f: stmt :=
+    "GVAR1" #= 1000 #;
+    Return "GVAR2"
+  .
+
+  Definition g: stmt :=
+    "GVAR2" #= 2000 #;
+    Return "GVAR1"
+  .
+
+  Definition main: stmt :=
+    (Call "f" []) #;
+    #assume ((Call "g" []) == 1000) #;
+    #assume ((Call "f" []) == 2000) #;
+    Put "Test(MultiModuleGenv) passed" Vnull
+  .
+
+  Definition main_function: function.
+    mk_function_tac main ([]:list var) ([]:list var). Defined.
+  Definition f_function: function. mk_function_tac f ([]: list var) ([]: list var). Defined.
+  Definition g_function: function. mk_function_tac g ([]: list var) ([]: list var). Defined.
+
+  Definition main_program: program := [("main", main_function)].
+  Definition f_program: program := [("f", f_function)].
+  Definition g_program: program := [("g", g_function)].
+
+  Definition modsems: list ModSem :=
+    List.map program_to_ModSem [main_program ; f_program ; g_program].
+
+  Definition isem: itree Event unit := eval_multimodule modsems.
+
+End MultiModuleGenv.
+
+
+
+
+
 Module MultiModuleLocalState.
 
   Inductive memoizeE: Type -> Type :=
   | GetM (k: nat): memoizeE (option nat)
   | SetM (k: nat) (v: nat): memoizeE unit
   .
-  Definition f_sem: CallExternalE ~> itree (CallExternalE +' Event +' memoizeE) :=
+  Definition f_sem: CallExternalE ~> itree (CallExternalE +' memoizeE +' GlobalE +' Event) :=
     (fun _ '(CallExternal func_name args) =>
        match args with
        | [Vnat k] =>
@@ -424,7 +565,7 @@ Module MultiModuleLocalState.
       then Some v
       else oh x
   .
-  Definition f_handler: memoizeE ~> stateT f_owned_heap (itree Event) :=
+  Definition f_handler: memoizeE ~> stateT f_owned_heap (itree (GlobalE +' Event)) :=
     fun T e oh =>
       match e with
       | GetM k => Ret (oh, oh k)
@@ -442,45 +583,46 @@ Module MultiModuleLocalState.
 
   Definition g x y r: stmt :=
     (#if x
-      then (y #:= (x - 1) #;
-              r #:= (Call "f" [CBV y]) #;
-              r #:= r + x)
-      else (r #:= 0)
+      then (y #= (x - 1) #;
+              r #= (Call "f" [CBV y]) #;
+              r #= r + x)
+      else (r #= 0)
     )
     #;
     Return r
   .
-  Definition g_function: function := mk_function ["x"] (g "x" "local0" "local1").
+  Definition g_function: function. mk_function_tac g ["x"] ["local0" ; "local1"]. Defined.
   Definition g_program: program := [("g", g_function)].
 
   Definition main r: stmt :=
-      r #:= (Call "f" [CBV 10]) #;
-      #put r #;
+      r #= (Call "f" [CBV 10]) #;
+      Put "" r #;
 
-      #put 99999 #;
-      #put 99999 #;
-      #put 99999 #;
+      Put "" 99999 #;
+      Put "" 99999 #;
+      Put "" 99999 #;
 
-      r #:= (Call "f" [CBV 10]) #;
-      #put r #;
+      r #= (Call "f" [CBV 10]) #;
+      Put "" r #;
 
-      #put 99999 #;
-      #put 99999 #;
-      #put 99999 #;
+      Put "" 99999 #;
+      Put "" 99999 #;
+      Put "" 99999 #;
 
-      r #:= (Call "f" [CBV 5]) #;
-      #put r #;
+      r #= (Call "f" [CBV 5]) #;
+      Put "" r #;
 
-      #put 99999 #;
-      #put 99999 #;
-      #put 99999 #;
+      Put "" 99999 #;
+      Put "" 99999 #;
+      Put "" 99999 #;
 
-      r #:= (Call "f" [CBV 8]) #;
-      #put r #;
+      r #= (Call "f" [CBV 8]) #;
+      Put "" r #;
 
       Skip
   .
-  Definition main_function: function := mk_function [] (main "local0").
+  Definition main_function: function.
+    mk_function_tac main ([]: list var) ["local0"]. Defined.
   Definition main_program: program := [("main", main_function)].
 
   Definition modsems: list ModSem :=
@@ -499,7 +641,7 @@ Module MultiModuleLocalStateSimple.
   | GetM: memoizeE (val)
   | SetM (v: val): memoizeE unit
   .
-  Definition f_sem: CallExternalE ~> itree (CallExternalE +' Event +' memoizeE) :=
+  Definition f_sem: CallExternalE ~> itree (CallExternalE +' memoizeE +' GlobalE +' Event) :=
     (fun _ '(CallExternal func_name args) =>
        match args with
        | [Vnat v] => trigger EYield ;; trigger (SetM v) ;; Ret (Vnull, [])
@@ -509,7 +651,7 @@ Module MultiModuleLocalStateSimple.
 
   Definition f_owned_heap: Type := val.
 
-  Definition f_handler: memoizeE ~> stateT f_owned_heap (itree Event) :=
+  Definition f_handler: memoizeE ~> stateT f_owned_heap (itree (GlobalE +' Event)) :=
     fun T e oh =>
       match e with
       | GetM => Ret (oh, oh)
@@ -528,28 +670,29 @@ Module MultiModuleLocalStateSimple.
   Definition g: stmt :=
     Return 10
   .
-  Definition g_function: function := mk_function [] (g).
+  Definition g_function: function. mk_function_tac g ([]: list var) ([]: list var). Defined.
   Definition g_program: program := [("g", g_function)].
 
   Definition main r: stmt :=
       (Call "f" [CBV 10]) #;
       (Call "g" []) #;
-      Yield #; r #:= (Call "f" []) #;
-      #if r == 10 then Skip else Assume #;
+      Yield #; r #= (Call "f" []) #;
+      #assume (r == 10) #;
       Debug "passed 1" Vnull #;
       (Call "g" []) #;
-      Yield #; r #:= (Call "f" []) #;
-      #if r == 10 then Skip else Assume #;
+      Yield #; r #= (Call "f" []) #;
+      #assume (r == 10) #;
       Debug "passed 2" Vnull #;
       Yield #; (Call "f" [CBV 20]) #;
       (Call "g" []) #;
-      Yield #; r #:= (Call "f" []) #;
-      #if r == 20 then Skip else Assume #;
+      Yield #; r #= (Call "f" []) #;
+      #assume (r == 20) #;
       Debug "passed 3" Vnull #;
       Put "Test(MultiModuleLocalStateSimple) passed" Vnull #;
       Skip
   .
-  Definition main_function: function := mk_function [] (main "local0").
+  Definition main_function: function.
+    mk_function_tac main ([]:list var) ["local0"]. Defined.
   Definition main_program: program := [("main", main_function)].
 
   Definition modsems1: list ModSem :=
@@ -566,96 +709,114 @@ End MultiModuleLocalStateSimple.
 
 
 
+Module MultiModuleMultiCore.
 
-Section RUN.
-Variable shuffle: forall A, list A -> list A.
+  Definition producer i: stmt :=
+    i #= 10 #;
+    #while i
+    do (
+      Debug "PRODUCER: " i #;
+      #if "GVAR" == 0
+       then ("GVAR" #= i #; i #= i-1)
+       else Skip #;
+      Yield
+    ) #;
+    "SIGNAL" #= "SIGNAL" + 1
+  .
 
-(* Definition rr_match {E R} `{Event -< E} *)
-(*            (rr : list (itree E R) -> itree E R) *)
-(*            (q:list (itree E R)) : itree E R *)
-(*   := *)
-(*     match q with *)
-(*     | [] => triggerUB *)
-(*     | t::ts => *)
-(*       match observe t with *)
-(*       | RetF _ => Tau (rr ts) *)
-(*       | TauF u => Tau (rr (u :: ts)) *)
-(*       | @VisF _ _ _ X o k => Vis o (fun x => rr (shuffle (k x :: ts))) *)
-(*       end *)
-(*     end. *)
+  Definition consumer s: stmt :=
+    s #= 0 #;
+    #while true
+    do (
+      Debug "CONSUMER: " s #;
+      #if "GVAR" == 0
+       then Skip
+       else s #= s + "GVAR" #;
+            "GVAR" #= 0
+      #;
+      #if "SIGNAL" == 2 then Break else Skip #;
+      Yield
+    ) #;
+    (* Put "" s #; *)
+    #assume (s == 110) #;
+    Put "Test(MultiCore3) passed" Vnull
+  .
 
-(* CoFixpoint round_robin {E R} `{Event -< e} (q:list (itree E R)) : itree E R := *)
-(*   rr_match round_robin q. *)
-Definition rr_match {R}
-           (rr : list (itree Event R) -> itree Event unit)
-           (q:list (itree Event R)) : itree Event unit
-  :=
-    match q with
-    | [] => Ret tt
-    | t::ts =>
-      match observe t with
-      | RetF _ => Tau (rr ts)
-      | TauF u => Tau (rr (u :: ts))
-      | @VisF _ _ _ X o k =>
-        match o with
-        | EYield => Vis o (fun x => rr (shuffle (k x :: ts)))
-        | _ => Vis o (fun x => rr (k x :: ts))
-        end
-        (* match o with *)
-        (* | Vis o (fun x => rr (shuffle (k x :: ts))) *)
-        (* (match o in Event Y return X = Y -> itree Event unit with *)
-        (* | EYield => fun pf => rr (k (eq_rect_r (fun T => T) tt pf) :: ts) *)
-        (* | _ => fun _ => Vis o (fun x => rr (k x :: ts)) *)
-        (* end) eq_refl *)
+  Definition producerF: function. mk_function_tac producer ([]: list var) (["i"]). Defined.
+  Definition consumerF: function. mk_function_tac consumer ([]: list var) (["s"]). Defined.
+
+  Definition producerP: program := [("producer", producerF) ].
+  Definition consumerP: program := [("consumer", consumerF) ].
+
+  Definition programs: list Lang.program := [ producerP ; consumerP ].
+  Definition modsems: list ModSem := List.map program_to_ModSem programs.
+
+  Definition sem: itree Event unit :=
+    eval_multimodule_multicore modsems [ "producer" ; "producer" ; "consumer" ].
+
+End MultiModuleMultiCore.
+
+
+Module MultiModuleMultiCoreLocalState.
+
+  Inductive memoizeE: Type -> Type :=
+  | GetM: memoizeE (val)
+  | SetM (v: val): memoizeE unit
+  .
+  Definition f_sem: CallExternalE ~> itree (CallExternalE +' memoizeE +' GlobalE +' Event) :=
+    (fun _ '(CallExternal func_name args) =>
+       match args with
+       | [Vnat v] => trigger EYield ;; trigger (SetM v) ;; Ret (Vnull, [])
+       | _ => trigger EYield ;; v <-  trigger (GetM) ;; Ret (v, [])
+       end)
+  .
+
+  Definition f_owned_heap: Type := val.
+
+  Definition f_handler: memoizeE ~> stateT f_owned_heap (itree (GlobalE +' Event)) :=
+    fun T e oh =>
+      match e with
+      | GetM => Ret (oh, oh)
+      | SetM v => Ret (v, tt)
       end
-    end.
+  .
+  Definition f_ModSem: ModSem :=
+    mk_ModSem
+      (fun s => string_dec s "f")
+      Vnull
+      memoizeE
+      f_handler
+      f_sem
+  .
 
-CoFixpoint round_robin {R} (q:list (itree Event R)) : itree Event unit :=
-  rr_match round_robin q.
+  Definition setter: stmt :=
+    (Call "f" [CBV 10]) #;
+    "SIGNAL" #= 1 #;
+    Skip
+  .
+
+  Definition getter: stmt :=
+    #while "SIGNAL" == 0 do Yield #;
+    #assume ((Call "f" []) == 10) #;
+    Put "Test(MultiModuleMultiCoreLocalState) passed" Vnull #;
+    Skip
+  .
+
+  Definition setterF: function.
+    mk_function_tac setter ([]:list var) ([]:list var). Defined.
+  Definition setterP: program := [("setter", setterF)].
+
+  Definition getterF: function.
+    mk_function_tac getter ([]:list var) ([]:list var). Defined.
+  Definition getterP: program := [("getter", getterF)].
+
+  Definition modsems: list ModSem :=
+    (List.map program_to_ModSem [setterP ; getterP]) ++ [f_ModSem]
+  .
+
+  Definition isem: itree Event unit :=
+    eval_multimodule_multicore modsems ["setter" ; "getter"].
+
+End MultiModuleMultiCoreLocalState.
 
 
-
-
-Variable handle_Event: forall E R X, Event X -> (X -> itree E R) -> itree E R.
-(* Extract Constant handle_Event => "handle_Event". *)
-
-Definition run_till_yield_aux {R} (rr : itree Event R -> (itree Event R))
-           (q: itree Event R) : (itree Event R)
-  :=
-    match observe q with
-    | RetF _ => q
-    | TauF u => Tau (rr u)
-      (* w <- (rr u) ;; (Tau w) *)
-    | @VisF _ _ _ X o k =>
-      (match o in Event Y return X = Y -> itree Event R with
-       | EYield => fun pf => k (eq_rect_r (fun T => T) tt pf)
-       | _ => (* fun _ => Vis o (fun x => rr (k x)) *)
-         fun _ => Tau (rr (handle_Event o k))
-       end) eq_refl
-      (* match o with *)
-      (* | EYield => Vis o (fun x => rr (k x)) *)
-      (* | _ => Vis o (fun x => rr (k x)) *)
-      (* end *)
-    (* Vis o (fun x => rr (shuffle (ts ++ [k x]))) *)
-    end.
-
-CoFixpoint run_till_yield {R} (q: itree Event R): (itree Event R) :=
-  run_till_yield_aux run_till_yield q
-.
-
-Definition is_ret {E R} (q: itree E R): bool := match observe q with RetF _ => true | _ => false end.
-
-Definition my_rr_match {R} (rr : list (itree Event R) -> list (itree Event R))
-           (q:list (itree Event R)) : list (itree Event R)
-  :=
-    match q with
-    | [] => []
-    | t::ts =>
-      let t2 := run_till_yield t in
-      rr (shuffle (List.filter (negb <*> is_ret) (t2::ts)))
-    end.
-
-Fail CoFixpoint my_round_robin {R} (q:list (itree Event R)) : list (itree Event R) :=
-  my_rr_match my_round_robin q.
-
-End RUN.
